Add mem in Sound.skenv, WIP on UnreachC.v

proof/AdequacySound.v
@@ -41,17 +41,17 @@ Section ADQSOUND.
 
   (* Let ge: Ge.t := sem_src.(Smallstep.globalenv). *)
 
-  Inductive sound_ge (su0: Sound.t): Prop :=
+  Inductive sound_ge (su0: Sound.t) (m0: mem): Prop :=
   | sound_ge_intro
-      (GE: Forall (fun ms => su0.(Sound.skenv) ms.(ModSem.skenv)) sem_src.(Smallstep.globalenv).(fst))
+      (GE: Forall (fun ms => su0.(Sound.skenv) m0 ms.(ModSem.skenv)) sem_src.(Smallstep.globalenv).(fst))
   .
 
   Lemma le_preserves_sound_ge
-        su0 su1
-        (GE: sound_ge su0)
+        m0 su0 su1
+        (GE: sound_ge su0 m0)
         (LE: Sound.le su0 su1)
     :
-      <<GE: sound_ge su1>>
+      <<GE: sound_ge su1 m0>>
   .
   Proof.
     inv GE.
@@ -60,9 +60,24 @@ Section ADQSOUND.
     ii. eapply Sound.skenv_le; eauto.
   Qed.
 
+  Lemma mle_preserves_sound_ge
+        m0 m1 su0
+        (GE: sound_ge su0 m0)
+        (LE: Sound.mle su0 m0 m1)
+    :
+      <<GE: sound_ge su0 m1>>
+  .
+  Proof.
+    inv GE.
+    econs; eauto.
+    rewrite Forall_forall in *.
+    ii. eapply Sound.skenv_mle; eauto.
+  Qed.
+
   (* stack can go preservation when su0 is given *)
   Inductive sound_stack (su0: Sound.t) (args: Args.t): list Frame.t -> Prop :=
   | sound_stack_nil
+      (GE: sound_ge su0 args.(Args.m))
     :
       sound_stack su0 args []
   | sound_stack_cons
@@ -90,7 +105,7 @@ Section ADQSOUND.
       )
       (GR: Sound.get_greatest su_tail args_tail su0)
       (EX: exists sound_state_ex, local_preservation ms sound_state_ex)
-      (GE: sound_ge su0)
+      (GE: sound_ge su0 args.(Args.m))
       (* sound_state_ex *)
       (* (PRSV: local_preservation ms sound_state_ex) *)
       (* (HD: sound_state_ex su0 lst0) *)
@@ -112,7 +127,7 @@ Section ADQSOUND.
           <<SUST: sound_state_all su0 m_arg lst0>>)
       (EX: exists sound_state_ex, local_preservation ms sound_state_ex)
       (ABCD: args_tail.(Args.m) = m_arg)
-      (GE: sound_ge su0)
+      (GE: sound_ge su0 m_arg)
     :
       sound_state su0 m_arg (State ((Frame.mk ms lst0) :: tail))
   | sound_state_call
@@ -121,7 +136,9 @@ Section ADQSOUND.
       (GR: Sound.get_greatest su_tail args su0)
       (ARGS: Sound.args su0 args)
       (STK: sound_stack su_tail args frs)
-      (GE: sound_ge su0)
+      (* (MLE: Sound.mle su0 m_tail args.(Args.m)) *)
+      (EQ: args.(Args.m) = m_tail)
+      (GE: sound_ge su0 m_tail)
     :
       sound_state su0 m_tail (Callstate args frs)
   .
@@ -129,9 +146,8 @@ Section ADQSOUND.
   Lemma sound_init
         st0
         (INIT: sem_src.(Smallstep.initial_state) st0)
-        m_init
     :
-      exists su0, sound_state su0 m_init st0
+      exists su0 m_init0, <<MEM: Sk.load_mem sk_link_src = Some m_init0>> /\ <<SU: sound_state su0 m_init0 st0>>
   .
   Proof.
     inv INIT. clarify. clear skenv_link_tgt p_tgt skenv_link_tgt sem_tgt LINKTGT.
@@ -140,17 +156,20 @@ Section ADQSOUND.
     { esplits; eauto. refl. }
     i; des.
     esplits; eauto.
-    econs; eauto.
-    - eapply Sound.greatest_adq; eauto.
-    - econs; eauto.
-    - econs. rewrite Forall_forall. intros ? IN. ss. des_ifs. u in IN.
-      eapply Sound.skenv_le; cycle 1; eauto.
-      { eapply Sound.greatest_adq; eauto. }
+    assert(GE: sound_ge su_init m_init).
+    {
+      econs. rewrite Forall_forall. intros ? IN. ss. des_ifs. u in IN.
       rewrite in_map_iff in IN.
       des; ss; clarify.
       + s. rewrite <- Sound.system_skenv; eauto.
       + eapply Sound.skenv_project; eauto.
         eapply Mod.get_modsem_projected_sk; eauto.
+    }
+    econs; eauto.
+    - eapply Sound.greatest_adq; eauto.
+    - econs; eauto.
+    - eapply le_preserves_sound_ge; eauto.
+      eapply Sound.greatest_adq; eauto.
   Unshelve.
     all: ss.
   Qed.
@@ -178,8 +197,15 @@ Section ADQSOUND.
       exists su_gr.
       exists args.(Args.m).
       esplits; eauto.
-      econs; eauto.
+      econs; eauto; swap 2 3.
       { eapply Sound.greatest_adq; eauto. }
+      { dup EX. inv EX. exploit CALL; eauto.
+        { eapply HD; eauto. }
+        i; des.
+        eapply le_preserves_sound_ge; eauto.
+        - eapply mle_preserves_sound_ge; eauto.
+        - eapply Sound.greatest_adq; eauto.
+      }
       econs; eauto.
       {
         ii. dup PRSV. bar. inv PRSV. exploit CALL; eauto; cycle 1.
@@ -191,7 +217,12 @@ Section ADQSOUND.
         }
         eapply HD; eauto.
       }
-      { eapply le_preserves_sound_ge; eauto. eapply Sound.greatest_adq; eauto. }
+      { eapply mle_preserves_sound_ge; eauto.
+        dup EX. inv EX. exploit CALL; eauto.
+        { eapply HD; eauto. }
+        i; des.
+        ss.
+      }
       (* intros ? ?. *)
       (* bar. dup PRSV. inv PRSV. bar. exploit CALL; eauto. { eapply HD; eauto. } i; des. *)
       (* dsplits; eauto. *)
@@ -238,8 +269,15 @@ Section ADQSOUND.
       bar.
       i; des.
       esplits; eauto. econs; try apply TL0; eauto.
-      ii. specialize (K sound_state_all PRSV).
-      eapply K; eauto.
+      + ii. specialize (K sound_state_all PRSV).
+        eapply K; eauto.
+      +
+        inv TL0; ss.
+        { eapply le_preserves_sound_ge; eauto.
+          eapply Sound.greatest_adq; eauto.
+        }
+        eapply le_preserves_sound_ge; eauto.
+        eapply Sound.greatest_adq; eauto.
   Unshelve.
     all: ss.
     admit "related to above admit".
